

likelihood:  $p(y|w) \propto \exp\left(-\frac{\beta}{2}(y - \Phi w)^T(y - \Phi w)\right)$

$$\Rightarrow \ln p(y|w) = -\frac{\beta}{2}(y^T y - 2y^T \Phi w + w^T \Phi^T \Phi w) + C$$

$$= -\frac{1}{2} w^T (\beta \Phi^T \Phi) w + w^T (\beta \Phi^T y) + C$$

prior:  $p(w) \propto \exp\left(-\frac{1}{2}(w - \mu_0)^T \Lambda_0 (w - \mu_0)\right)$

$$\Rightarrow \ln p(w) = -\frac{1}{2} w^T (\Lambda_0) w + w^T (\Lambda_0 \mu_0) + C$$

posterior:  $\ln p(w|y) = \ln p(y|w) + \ln p(w)$

$$= -\frac{1}{2} w^T (\beta \Phi^T \Phi + \Lambda_0) w + w^T (\beta \Phi^T y + \Lambda_0 \mu_0) + C$$

$$\ln p(w|y) = \ln N(w | \mu_N, \Lambda_N^{-1})$$

$$= -\frac{1}{2} (w - \mu_N)^T \Lambda_N (w - \mu_N) + C$$

$$= -\frac{1}{2} w^T \Lambda_N w + w^T \Lambda_N \mu_N + C$$

二次项:  $\Lambda_N = \Lambda_0 + \beta \Phi^T \Phi$

一次项:  $\Lambda_N \mu_N = \Lambda_0 \mu_0 + \beta \Phi^T y$

$\therefore \Lambda_N = \Lambda_0 + \beta \Phi^T \Phi$

$\Rightarrow \begin{cases} \mu_N = \Lambda_N^{-1} (\Lambda_0 \mu_0 + \beta \Phi^T y) \\ S_N = \Lambda_N^{-1} = (\Lambda_0 + \beta \Phi^T \Phi)^{-1} \end{cases}$